update

theory/Dynamic_Communication_Analysis.thy
@@ -4,59 +4,58 @@ begin
 
 inductive is_send_path :: "trace_pool \<Rightarrow> chan \<Rightarrow> control_path \<Rightarrow> bool" where
   Intro: "
-    \<E> \<pi>\<^sub>y = Some (\<langle>LET x\<^sub>y = SYNC x\<^sub>e in e\<^sub>n; \<rho>; \<kappa>\<rangle>) \<Longrightarrow>
-    \<rho> x\<^sub>e = Some (VClosure (Send_Evt x\<^sub>s\<^sub>c x\<^sub>m) \<rho>\<^sub>e) \<Longrightarrow>
-    \<rho>\<^sub>e x\<^sub>s\<^sub>c = Some (VChan c) \<Longrightarrow>
-    is_send_path \<E> c \<pi>\<^sub>y
+    trpl \<pi>y = Some (\<langle>LET xy = SYNC xe in en; env; \<kappa>\<rangle>) \<Longrightarrow>
+    env xe = Some (VClosure (Send_Evt xsc xm) enve) \<Longrightarrow>
+    enve xsc = Some (VChan c) \<Longrightarrow>
+    is_send_path trpl c \<pi>y
   "
 
 inductive is_recv_path :: "trace_pool \<Rightarrow> chan \<Rightarrow> control_path \<Rightarrow> bool" where
   Intro: "
-    \<E> \<pi>\<^sub>y = Some (\<langle>LET x\<^sub>y = SYNC x\<^sub>e in e\<^sub>n; \<rho>; \<kappa>\<rangle>) \<Longrightarrow>
-    \<rho> x\<^sub>e = Some (VClosure (Recv_Evt x\<^sub>r\<^sub>c) \<rho>\<^sub>e) \<Longrightarrow>
-    \<rho>\<^sub>e x\<^sub>r\<^sub>c = Some (VChan c) \<Longrightarrow>
-    is_recv_path \<E> c \<pi>\<^sub>y
+    trpl \<pi>y = Some (\<langle>LET xy = SYNC xe in en; env; \<kappa>\<rangle>) \<Longrightarrow>
+    env xe = Some (VClosure (Recv_Evt xrc) enve) \<Longrightarrow>
+    enve xrc = Some (VChan c) \<Longrightarrow>
+    is_recv_path trpl c \<pi>y
   "
 
 
 inductive every_two_dynamic_paths  :: "(control_path \<Rightarrow> bool) \<Rightarrow> (control_path \<Rightarrow> control_path \<Rightarrow> bool) \<Rightarrow> bool" where
   "
-    (\<forall> \<pi>\<^sub>1 \<pi>\<^sub>2 .
-      P \<pi>\<^sub>1 \<longrightarrow>
-      P \<pi>\<^sub>2 \<longrightarrow>
-      R \<pi>\<^sub>1 \<pi>\<^sub>2
+    (\<forall> \<pi>1 \<pi>2 .
+      P \<pi>1 \<longrightarrow>
+      P \<pi>2 \<longrightarrow>
+      R \<pi>1 \<pi>2
     ) \<Longrightarrow>
     every_two_dynamic_paths P R
   "
 
-fun ordered where
-  "ordered \<pi>\<^sub>1 \<pi>\<^sub>2 = (prefix \<pi>\<^sub>1 \<pi>\<^sub>2 \<or> prefix \<pi>\<^sub>2 \<pi>\<^sub>1)"
+inductive ordered :: "'a list \<Rightarrow> 'a list \<Rightarrow> bool" where
+  left: "prefix \<pi>1 \<pi>2 \<Longrightarrow> ordered \<pi>1 \<pi>2" |
+  right: "prefix \<pi>2 \<pi>1 \<Longrightarrow> ordered \<pi>1 \<pi>2"
 
 inductive one_shot :: "trace_pool \<Rightarrow> chan \<Rightarrow> bool" where
   "
-    every_two_dynamic_paths (is_send_path \<E> c) op= \<Longrightarrow> 
-    one_shot \<E> c
+    every_two_dynamic_paths (is_send_path trpl c) op= \<Longrightarrow> 
+    one_shot trpl c
   "
-
-
-inductive one_to_one :: "trace_pool \<Rightarrow> chan \<Rightarrow> bool" where
-  "
-    every_two_dynamic_paths (is_send_path \<E> c) ordered \<and> every_two_dynamic_paths (is_recv_path \<E> c) ordered \<Longrightarrow> 
-    one_to_one \<E> c
-  "
-  
 
 inductive fan_out :: "trace_pool \<Rightarrow> chan \<Rightarrow> bool" where
+  Intro: "
+    every_two_dynamic_paths (is_send_path trpl c) ordered \<Longrightarrow>
+    fan_out trpl c
   "
-    every_two_dynamic_paths (is_send_path \<E> c) ordered \<Longrightarrow>
-    fan_out \<E> c
-  "
-
   
 inductive fan_in :: "trace_pool \<Rightarrow> chan \<Rightarrow> bool" where
+  Intro: "
+    every_two_dynamic_paths (is_recv_path trpl c) ordered \<Longrightarrow> 
+    fan_in trpl c
   "
-    every_two_dynamic_paths (is_recv_path \<E> c) ordered \<Longrightarrow> 
-    fan_in \<E> c
+
+inductive one_to_one :: "trace_pool \<Rightarrow> chan \<Rightarrow> bool" where
+  Intro: "
+    fan_out trpl c \<Longrightarrow>
+    fan_in trpl c \<Longrightarrow> 
+    one_to_one trpl c
   "
 
 
